stage0/stdlib/Init/Data/Nat/Div.c
@@ -1,6 +1,6 @@
 // Lean compiler output
 // Module: Init.Data.Nat.Div
-// Imports: Init.WF Init.Data.Nat.Basic
+// Imports: Init.WF Init.WFTactics Init.Data.Nat.Basic
 #include <lean/lean.h>
 #if defined(__clang__)
 #pragma clang diagnostic ignored "-Wunused-parameter"
@@ -16,67 +16,11 @@ extern "C" {
 static lean_object* l_Nat_instDivNat___closed__1;
 lean_object* lean_nat_div(lean_object*, lean_object*);
 LEAN_EXPORT lean_object* l_Nat_div___boxed(lean_object*, lean_object*);
-lean_object* lean_nat_add(lean_object*, lean_object*);
-lean_object* lean_nat_sub(lean_object*, lean_object*);
-LEAN_EXPORT lean_object* l___private_Init_Data_Nat_Div_0__Nat_mod_F(lean_object*, lean_object*, lean_object*);
 LEAN_EXPORT lean_object* l_Nat_mod___boxed(lean_object*, lean_object*);
-LEAN_EXPORT lean_object* l___private_Init_Data_Nat_Div_0__Nat_div_F___boxed(lean_object*, lean_object*, lean_object*);
 LEAN_EXPORT lean_object* l_Nat_instModNat;
-uint8_t lean_nat_dec_le(lean_object*, lean_object*);
-LEAN_EXPORT lean_object* l___private_Init_Data_Nat_Div_0__Nat_div_F(lean_object*, lean_object*, lean_object*);
-LEAN_EXPORT lean_object* l___private_Init_Data_Nat_Div_0__Nat_mod_F___boxed(lean_object*, lean_object*, lean_object*);
 LEAN_EXPORT lean_object* l_Nat_instDivNat;
 lean_object* lean_nat_mod(lean_object*, lean_object*);
 static lean_object* l_Nat_instModNat___closed__1;
-uint8_t lean_nat_dec_lt(lean_object*, lean_object*);
-LEAN_EXPORT lean_object* l___private_Init_Data_Nat_Div_0__Nat_div_F(lean_object* x_1, lean_object* x_2, lean_object* x_3) {
-_start:
-{
-lean_object* x_4; uint8_t x_5; 
-x_4 = lean_unsigned_to_nat(0u);
-x_5 = lean_nat_dec_lt(x_4, x_3);
-if (x_5 == 0)
-{
-lean_object* x_6; 
-lean_dec(x_3);
-lean_dec(x_2);
-x_6 = lean_unsigned_to_nat(0u);
-return x_6;
-}
-else
-{
-uint8_t x_7; 
-x_7 = lean_nat_dec_le(x_3, x_1);
-if (x_7 == 0)
-{
-lean_object* x_8; 
-lean_dec(x_3);
-lean_dec(x_2);
-x_8 = lean_unsigned_to_nat(0u);
-return x_8;
-}
-else
-{
-lean_object* x_9; lean_object* x_10; lean_object* x_11; lean_object* x_12; 
-x_9 = lean_nat_sub(x_1, x_3);
-x_10 = lean_apply_3(x_2, x_9, lean_box(0), x_3);
-x_11 = lean_unsigned_to_nat(1u);
-x_12 = lean_nat_add(x_10, x_11);
-lean_dec(x_10);
-return x_12;
-}
-}
-}
-}
-LEAN_EXPORT lean_object* l___private_Init_Data_Nat_Div_0__Nat_div_F___boxed(lean_object* x_1, lean_object* x_2, lean_object* x_3) {
-_start:
-{
-lean_object* x_4; 
-x_4 = l___private_Init_Data_Nat_Div_0__Nat_div_F(x_1, x_2, x_3);
-lean_dec(x_1);
-return x_4;
-}
-}
 LEAN_EXPORT lean_object* l_Nat_div___boxed(lean_object* x_1, lean_object* x_2) {
 _start:
 {
@@ -101,49 +45,6 @@ _start:
 lean_object* x_1; 
 x_1 = l_Nat_instDivNat___closed__1;
 return x_1;
-}
-}
-LEAN_EXPORT lean_object* l___private_Init_Data_Nat_Div_0__Nat_mod_F(lean_object* x_1, lean_object* x_2, lean_object* x_3) {
-_start:
-{
-lean_object* x_4; uint8_t x_5; 
-x_4 = lean_unsigned_to_nat(0u);
-x_5 = lean_nat_dec_lt(x_4, x_3);
-if (x_5 == 0)
-{
-lean_dec(x_3);
-lean_dec(x_2);
-lean_inc(x_1);
-return x_1;
-}
-else
-{
-uint8_t x_6; 
-x_6 = lean_nat_dec_le(x_3, x_1);
-if (x_6 == 0)
-{
-lean_dec(x_3);
-lean_dec(x_2);
-lean_inc(x_1);
-return x_1;
-}
-else
-{
-lean_object* x_7; lean_object* x_8; 
-x_7 = lean_nat_sub(x_1, x_3);
-x_8 = lean_apply_3(x_2, x_7, lean_box(0), x_3);
-return x_8;
-}
-}
-}
-}
-LEAN_EXPORT lean_object* l___private_Init_Data_Nat_Div_0__Nat_mod_F___boxed(lean_object* x_1, lean_object* x_2, lean_object* x_3) {
-_start:
-{
-lean_object* x_4; 
-x_4 = l___private_Init_Data_Nat_Div_0__Nat_mod_F(x_1, x_2, x_3);
-lean_dec(x_1);
-return x_4;
 }
 }
 LEAN_EXPORT lean_object* l_Nat_mod___boxed(lean_object* x_1, lean_object* x_2) {
@@ -173,6 +74,7 @@ return x_1;
 }
 }
 lean_object* initialize_Init_WF(uint8_t builtin, lean_object*);
+lean_object* initialize_Init_WFTactics(uint8_t builtin, lean_object*);
 lean_object* initialize_Init_Data_Nat_Basic(uint8_t builtin, lean_object*);
 static bool _G_initialized = false;
 LEAN_EXPORT lean_object* initialize_Init_Data_Nat_Div(uint8_t builtin, lean_object* w) {
@@ -180,6 +82,9 @@ lean_object * res;
 if (_G_initialized) return lean_io_result_mk_ok(lean_box(0));
 _G_initialized = true;
 res = initialize_Init_WF(builtin, lean_io_mk_world());
+if (lean_io_result_is_error(res)) return res;
+lean_dec_ref(res);
+res = initialize_Init_WFTactics(builtin, lean_io_mk_world());
 if (lean_io_result_is_error(res)) return res;
 lean_dec_ref(res);
 res = initialize_Init_Data_Nat_Basic(builtin, lean_io_mk_world());
