stage0/src/Init/Core.lean
@@ -262,6 +262,22 @@ theorem true_ne_false : ¬True = False :=
 
 end Ne
 
+theorem Bool.of_not_eq_true : {b : Bool} → ¬ (b = true) → b = false
+  | true,  h => absurd rfl h
+  | false, h => rfl
+
+theorem Bool.of_not_eq_false : {b : Bool} → ¬ (b = false) → b = true
+  | true,  h => rfl
+  | false, h => absurd rfl h
+
+theorem ne_of_beq_false [BEq α] [LawfulBEq α] {a b : α} (h : (a == b) = false) : a ≠ b := by
+  intro h'; subst h'; have : true = false := Eq.trans (LawfulBEq.rfl a).symm h; contradiction
+
+theorem beq_false_of_ne [BEq α] [LawfulBEq α] {a b : α} (h : a ≠ b) : (a == b) = false :=
+  have : ¬ (a == b) = true := by
+    intro h'; rw [eq_of_beq h'] at h; contradiction
+  Bool.of_not_eq_true this
+
 section
 variable {α β φ : Sort u} {a a' : α} {b b' : β} {c : φ}
 
